Add tracker implementation

theories/Dynamics/Procedure.v
@@ -1,163 +1,150 @@
-From stdpp Require Import base list stringmap gmap fin_maps.
 From Metaconfigurations.Syntax Require Import Value Term Stmt.
 
 From Metaconfigurations Require Import 
   Map Syntax.Term Syntax.Stmt
   Syntax.Value
   Dynamics.Term Object.
-From stdpp Require Import base.
-Require Import Coq.ZArith.BinInt.
 
 From Metaconfigurations.Dynamics Require Import Term Stmt.
+From stdpp Require Import base list stringmap gmap fin_maps.
 
+Record procedure (Π Ω : Type) `{Object Π Ω} := {
+  param : string;
+  body : list (Stmt.t Π Ω);
+}.
 
-Section Procedure.
-  Variable Π : Type.
+Arguments param {_ _ _ _}.
+Arguments body {_ _ _ _}.
 
-  Context `{Countable Π}.
+Record frame (Π Ω : Type) `{Object Π Ω} := {
+  pc : nat;
+  registers : stringmap Value.t;
+  proc : procedure Π Ω;
+}.
 
-  (* Type of implemented object *)
-  Variable Ω₀ : Type.
+Arguments pc {_ _ _ _}.
+Arguments registers {_ _ _ _}.
+Arguments proc {_ _ _ _}.
 
-  (* The object being implemented *)
-  Context {ω : Ω₀}.
+Variant signal (Π Ω : Type) `{Object Π Ω} :=
+  | Next (f : frame Π Ω) (* On next step, go to line [l] *)
+  | Return (v : Value.t). (* Procedure has returned with value [v] *)
 
-  Context `{Object Π Ω₀}.
+Arguments Next {_ _ _ _}.
+Arguments Return {_ _ _ _}.
 
-  (* Set of base objects *)
-  Variable Ω : Type.
+Record Implementation (Π Ω : Type) {Ω} `{Object Π Ω₀, Object Π Ω} (ω : Ω₀) := {
+  (* Initial states for every base object *)
+  initial_states : states Π Ω;
+  (* Assignment from every process π and operation OP to a procedure *)
+  procedures : (type ω).(OP) → procedure Π Ω;
+}.
 
-  (* Context `{EqDecision Ω}. *)
+Arguments initial_states : default implicits.
+Arguments procedures : default implicits.
 
-  Context `{Object Π Ω}.
+Local Open Scope dynamics_scope.
 
-  Record procedure := {
-    param : string;
-    body : list (Stmt.t Π Ω);
-  }.
+Variant step_procedure {Π Ω} `{Object Π Ω} (π : Π) : states Π Ω → frame Π Ω → states Π Ω → signal Π Ω → Prop :=
+  | step_next pc pc' s ψ ψ' proc ϵ ϵ' :
+    (* If [pc] points to line containing statement [s] in [proc] *)
+    proc.(body) !! pc = Some s →
+    ⟨ π , ψ , ϵ , s ⟩ ⇓ₛ ⟨ ψ' , ϵ' , Goto pc' ⟩ →
+    step_procedure π ϵ {| pc := pc; registers := ψ; proc := proc |} ϵ' (Next {| pc := pc'; registers := ψ'; proc := proc |})
+  | step_implicit_return pc ψ proc ϵ :
+    (* Control has fallen off end of procedure *)
+    proc.(body) !! pc = None →
+    step_procedure π ϵ {| pc := pc; registers := ψ; proc := proc |} ϵ (Return ⊤ᵥ)
+  | step_return pc s ψ proc ϵ ϵ' v:
+    proc.(body) !! pc = Some s →
+    ⟨ π , ψ , ϵ , s ⟩ ⇓ₛ ⟨ ψ , ϵ' , Stmt.Return v ⟩ →
+    step_procedure π ϵ {| pc := pc; registers := ψ; proc := proc |} ϵ (Return v).
 
-  Record Implementation := {
-    (* Initial states for every base object *)
-    initial_states : states Π Ω;
-    (* Assignment from every process π and operation OP to a procedure *)
-    procedures : (type ω).(OP Π) → procedure;
-  }.
+Record configuration (Π Ω : Type) `{Countable Π, Object Π Ω} := {
+  outstanding : gmap Π (frame Π Ω);
+  ϵ : states Π Ω;
+}.
 
-  Record frame := {
-    pc : nat;
-    registers : stringmap Value.t;
-    proc : procedure;
-  }.
+Arguments outstanding {_ _ _ _ _ _ _}.
+Arguments ϵ {_ _ _ _ _ _ _}.
 
-  Variant signal :=
-    | Next (f : frame) (* On next step, go to line [l] *)
-    | Return (v : Value.t) (* Procedure has returned with value [v] *).
+Variant line Π {Ω} `{Object Π Ω} (ω : Ω) :=
+  | Invoke (op : (type ω).(OP)) (arg : Value.t)
+  | Intermediate
+  | Response (resp : Value.t).
 
-  Local Open Scope dynamics_scope.
+Arguments Invoke {_ _ _ _ _}.
+Arguments Intermediate {_ _ _ _ _}.
+Arguments Response {_ _ _ _ _}.
 
-  Variant step_procedure (π : Π) : states Π Ω → frame → states Π Ω → signal → Prop :=
-    | step_next pc pc' s ψ ψ' proc ϵ ϵ' :
-      (* If [pc] points to line containing statement [s] in [proc] *)
-      proc.(body) !! pc = Some s →
-      ⟨ π , ψ , ϵ , s ⟩ ⇓ₛ ⟨ ψ' , ϵ' , Goto pc' ⟩ →
-      step_procedure π ϵ {| pc := pc; registers := ψ; proc := proc |} ϵ' (Next {| pc := pc'; registers := ψ'; proc := proc |})
-    | step_implicit_return pc ψ proc ϵ :
-      (* Control has fallen off end of procedure *)
-      proc.(body) !! pc = None →
-      step_procedure π ϵ {| pc := pc; registers := ψ; proc := proc |} ϵ (Return ⊤ᵥ)
-    | step_return pc s ψ proc ϵ ϵ' v:
-      proc.(body) !! pc = Some s →
-      ⟨ π , ψ , ϵ , s ⟩ ⇓ₛ ⟨ ψ , ϵ' , Stmt.Return v ⟩ →
-      step_procedure π ϵ {| pc := pc; registers := ψ; proc := proc |} ϵ (Return v).
+Inductive run Π {Ω} `{Countable Π, Object Π Ω} (ω : Ω) :=
+  | Initial (c : configuration Π Ω)
+  | Step (r : run Π ω) (π : Π) (l : line Π ω) (c : configuration Π Ω).
 
-  Record configuration := {
-    outstanding : gmap Π frame;
-    ϵ : states Π Ω;
-  }.
+Arguments Initial {_ _ _ _ _ _ _}.
+Arguments Step {_ _ _ _ _ _ _}.
 
-  Variant line :=
-    | Invoke (op : (type ω).(OP Π)) (arg : Value.t)
-    | Intermediate
-    | Response (resp : Value.t).
+Section Run.
 
-  Inductive run :=
-    | Initial (c : configuration)
-    | Step (r : run) (π : Π) (l : line) (c : configuration).
+  Context {Π Ω₀ Ω} `{Countable Π, Object Π Ω₀, Object Π Ω} {ω : Ω}.
 
-  Section Run.
+  Variable impl : Implementation Π Ω ω.
 
-    Variable impl : Implementation.
+  Definition initial_frame op arg :=
+    let proc := procedures impl op in
+    {|
+      pc := 0;
+      registers := singletonM proc.(param) arg;
+      proc := proc;
+    |}.
 
-    Definition initial_frame op arg :=
-      let proc := procedures impl op in
-      {|
-        pc := 0;
-        registers := singletonM proc.(param) arg;
-        proc := proc;
-      |}.
+  Variant step : configuration Π Ω → Π → line Π ω → configuration Π Ω → Prop :=
+    | step_invoke outstanding π ϵ ϵ' op arg f :
+      outstanding !! π = None →
+      step_procedure π ϵ (initial_frame op arg) ϵ' (Next f) →
+      step {| outstanding := outstanding; ϵ := ϵ |} π (Invoke op arg) {| outstanding := <[π := f]>outstanding; ϵ := ϵ' |}
+    | step_intermediate outstanding π ϵ ϵ' f f' :
+    (* If process [π] has an outstanding request for proecedure [proc], interrupted at line [pc] *)
+      outstanding !! π = Some f →
+      step_procedure π ϵ f ϵ' (Next f') →
+      step {| outstanding := outstanding; ϵ := ϵ |} π Intermediate {| outstanding := <[π := f']>outstanding; ϵ := ϵ' |}
+    | step_response outstanding π ϵ ϵ' f v :
+    (* If process [π] has an outstanding request for proecedure [proc], interrupted at line [pc] *)
+      outstanding !! π = Some f →
+      step_procedure π ϵ f ϵ' (Return v) →
+      step {| outstanding := outstanding; ϵ := ϵ |} π (Response v) {| outstanding := delete π outstanding; ϵ := ϵ' |}.
 
-    Variant step : configuration → Π → line → configuration → Prop :=
-      | step_invoke outstanding π ϵ ϵ' op arg f :
-        outstanding !! π = None →
-        step_procedure π ϵ (initial_frame op arg) ϵ' (Next f) →
-        step {| outstanding := outstanding; ϵ := ϵ |} π (Invoke op arg) {| outstanding := <[π := f]>outstanding; ϵ := ϵ' |}
-      | step_intermediate outstanding π ϵ ϵ' f f' :
-      (* If process [π] has an outstanding request for proecedure [proc], interrupted at line [pc] *)
-        outstanding !! π = Some f →
-        step_procedure π ϵ f ϵ' (Next f') →
-        step {| outstanding := outstanding; ϵ := ϵ |} π Intermediate {| outstanding := <[π := f']>outstanding; ϵ := ϵ' |}
-      | step_response outstanding π ϵ ϵ' f v :
-      (* If process [π] has an outstanding request for proecedure [proc], interrupted at line [pc] *)
-        outstanding !! π = Some f →
-        step_procedure π ϵ f ϵ' (Return v) →
-        step {| outstanding := outstanding; ϵ := ϵ |} π (Response v) {| outstanding := delete π outstanding; ϵ := ϵ' |}.
+  Definition final (r : run Π ω) :=
+    match r with
+    | Initial c | Step _ _ _ c => c
+    end.
 
-    Definition final r :=
-      match r with
-      | Initial c | Step _ _ _ c => c
-      end.
+  Inductive Run : run Π ω → Prop :=
+    | Run_initial : Run (Initial {| outstanding := ∅; ϵ := impl.(initial_states) |})
+    | Run_step r π l c : Run r → step (final r) π l c → Run (Step r π l c).
 
-    Inductive Run : run → Prop :=
-      | Run_initial : Run (Initial {| outstanding := ∅; ϵ := impl.(initial_states) |})
-      | Run_step r π l c : Run r → step (final r) π l c → Run (Step r π l c).
+  Fixpoint behavior (r : run Π ω) : list (Π * line Π ω) :=
+    match r with
+    | Initial _ => []
+    | Step r π l c =>
+        match l with
+        | Invoke _ _ | Response _ => (π, l) :: behavior r
+        | Intermediate => behavior r
+        end
+    end.
 
-    Fixpoint behavior r : list (Π * line) :=
-      match r with
-      | Initial _ => []
-      | Step r π l c =>
-          match l with
-          | Invoke _ _ | Response _ => behavior r ++ [(π, l)]
-          | Intermediate => behavior r
-          end
-      end.
+  Variant Behavior : list (Π * line Π ω) → Prop :=
+    | Behavior_intro (r : run Π ω) : Run r → Behavior (behavior r).
 
-    Variant Behavior : list (Π * line) → Prop :=
-      | Behavior_intro (r : run) : Run r → Behavior (behavior r).
+  Lemma behavior_no_intermediate π l r : Behavior r → (π, l) ∈ r → l ≠ Intermediate.
+  Proof.
+  Admitted.
 
-    Lemma behavior_no_intermediate π l r : Behavior r → (π, l) ∈ r → l ≠ Intermediate.
-    Proof.
-    Admitted.
+End Run.
 
-  End Run.
+Section LiftL.
 
-End Procedure.
-
-Section Augmentation.
-
-  Variable Π : Type.
-
-  Context `{Countable Π}.
-
-  (* Type of implemented object *)
-  Variable Ω₀ : Type.
-
-  (* The object being implemented *)
-  Variable ω : Ω₀.
-
-  Context `{Object Π Ω₀}.
-
-  (* Set of base objects *)
-  Variable Ω : Type.
+  Context {Π Ω : Type}.
 
   Context `{Object Π Ω}.
 
@@ -191,10 +178,10 @@ Section Augmentation.
       ⟨ π , ψ , ϵ₁ , e ⟩ ⇓ₑ ⟨ ϵ₁' , v ⟩ →
         ⟨ π , ψ , disjoint_union ϵ₁ ϵ₂ , lift_term_l e ⟩ ⇓ₑ ⟨ disjoint_union ϵ₁' ϵ₂ , v ⟩.
   Proof.
-    induction e; intros; simpl in *; inv H3; try (econstructor; eauto).
+    induction e; intros; simpl in *; inv H1; try (econstructor; eauto).
     rewrite rebind_union_distr_l. econstructor.
       + eapply IHe. eauto.
-      + inv H10. econstructor. unfold Map.lookup in *. simpl in *. assumption.
+      + inv H8. econstructor. unfold Map.lookup in *. simpl in *. assumption.
   Qed.
 
   Lemma lift_term_l_sound_l :
@@ -202,12 +189,12 @@ Section Augmentation.
       ⟨ π , ψ , ϵ , lift_term_l e ⟩ ⇓ₑ ⟨ ϵ' , v ⟩ →
         ⟨ π , ψ , πₗ ϵ , e ⟩ ⇓ₑ ⟨ πₗ ϵ' , v ⟩.
   Proof.
-    induction e; intros; simpl in *; inv H3; try (econstructor; eauto).
+    induction e; intros; simpl in *; inv H1; try (econstructor; eauto).
     rewrite πₗ_rebind_comm. econstructor.
     + apply IHe. eassumption.
-    + inv H10. constructor. simpl in *.
-      replace (Map.lookup ω0 (πₗ ϵ0)) 
-          with (Map.lookup (inl ω0) ϵ0) by reflexivity.
+    + inv H8. constructor. simpl in *.
+      replace (Map.lookup ω (πₗ ϵ0)) 
+          with (Map.lookup (inl ω) ϵ0) by reflexivity.
       assumption.
   Qed.
 
@@ -215,14 +202,14 @@ Section Augmentation.
     ∀ e π ψ ϵ v ϵ',
       ⟨ π , ψ , ϵ , lift_term_l e ⟩ ⇓ₑ ⟨ ϵ' , v ⟩ → πᵣ ϵ = πᵣ ϵ'.
   Proof.
-    induction e; intros; simpl in *; inv H3; intuition.
-    - apply IHe in H9. subst. simpl in *.
+    induction e; intros; simpl in *; inv H1; intuition.
+    - apply IHe in H7. subst. simpl in *.
       replace (πᵣ ϵ0) with (πᵣ ϵ'0). apply rebind_l_πᵣ.
-    - apply IHe1 in H7. apply IHe2 in H10. congruence.
-    - inv H9. eauto.
-    - apply IHe1 in H6. apply IHe2 in H9. congruence.
-    - apply IHe in H5. assumption.
-    - apply IHe in H5. assumption.
+    - apply IHe1 in H5. apply IHe2 in H8. congruence.
+    - inv H7. eauto.
+    - apply IHe1 in H4. apply IHe2 in H7. congruence.
+    - apply IHe in H3. assumption.
+    - apply IHe in H3. assumption.
   Qed.
 
   Fixpoint lift_stmt_l (s : Stmt.t Π Ω) : Stmt.t Π (Ω + Ω') :=
@@ -242,7 +229,7 @@ Section Augmentation.
         ∀ ϵ₂,
           ⟨ π , ψ , disjoint_union ϵ₁ ϵ₂ , lift_stmt_l s ⟩ ⇓ₛ ⟨ ψ' , disjoint_union ϵ₁' ϵ₂ , sig ⟩.
   Proof.
-    intros. generalize dependent ϵ₂. induction H3; intros.
+    intros. generalize dependent ϵ₂. induction H1; intros.
     - econstructor.
     - econstructor. fold lift_stmt_l. eauto.
     - econstructor. eauto.
@@ -253,7 +240,7 @@ Section Augmentation.
       + fold lift_stmt_l. eapply IHeval.
     - econstructor. eapply lift_term_l_complete. eassumption.
     - econstructor.
-    - econstructor. eapply lift_term_l_complete in H3. eauto.
+    - econstructor. eapply lift_term_l_complete in H1. eauto.
     - econstructor. eapply lift_term_l_complete. eassumption.
   Qed.
 
@@ -263,19 +250,19 @@ Section Augmentation.
         ⟨ π , ψ , πₗ ϵ , s ⟩ ⇓ₛ ⟨ ψ' , πₗ ϵ' , sig ⟩.
   Proof.
     induction s; intros.
-    - inv H3; econstructor; eauto.
-    - inv H3. econstructor. eapply lift_term_l_sound_l. eassumption.
-    - inv H3.
+    - inv H1; econstructor; eauto.
+    - inv H1. econstructor. eapply lift_term_l_sound_l. eassumption.
+    - inv H1.
       + econstructor.
         * eapply lift_term_l_sound_l. eassumption.
         * eauto.
       + eapply eval_if_false.
         * eapply lift_term_l_sound_l. eassumption.
         * eauto.
-    - inv H3. econstructor.
-    - inv H3. econstructor. eapply lift_term_l_sound_l. assumption.
-    - simpl in *. destruct inv. inv H3. econstructor. eapply lift_term_l_sound_l. simpl. eassumption.
-    - inv H3. econstructor.
+    - inv H1. econstructor.
+    - inv H1. econstructor. eapply lift_term_l_sound_l. assumption.
+    - simpl in *. destruct inv. inv H1. econstructor. eapply lift_term_l_sound_l. simpl. eassumption.
+    - inv H1. econstructor.
   Qed.
 
   Lemma lift_stmt_l_sound_r :
@@ -283,28 +270,40 @@ Section Augmentation.
       ⟨ π , ψ , ϵ , lift_stmt_l s ⟩ ⇓ₛ ⟨ ψ' , ϵ' , sig ⟩ → πᵣ ϵ = πᵣ ϵ'.
   Proof.
     induction s; intros.
-    - inv H3.
+    - inv H1.
       + eauto.
       + eauto.
       + etransitivity.
         * eapply IHs1. eauto.
         * eauto.
-    - inv H3. reflexivity.
-    - inv H3.
+    - inv H1. reflexivity.
+    - inv H1.
       + etransitivity.
         * eapply lift_term_l_sound_r. eassumption.
         * eauto.
       + etransitivity.
         * eapply lift_term_l_sound_r. eassumption.
         * eauto.
-    - inv H3. econstructor.
-    - inv H3. eapply lift_term_l_sound_r. eassumption.
-    - cbn in *. destruct inv. inv H3. eapply lift_term_l_sound_r.
-      assert (Term.Invoke (inl ω0) op (lift_term_l arg) = lift_term_l (Term.Invoke ω0 op arg)) by reflexivity.
-      erewrite <- H3.
+    - inv H1. econstructor.
+    - inv H1. eapply lift_term_l_sound_r. eassumption.
+    - cbn in *. destruct inv. inv H1. eapply lift_term_l_sound_r.
+      assert (Term.Invoke (inl ω) op (lift_term_l arg) = lift_term_l (Term.Invoke ω op arg)) by reflexivity.
+      erewrite <- H1.
       eassumption.
-    - inv H3. econstructor.
+    - inv H1. econstructor.
   Qed.
+
+End LiftL.
+
+Section LiftR.
+
+  Context {Π Ω' : Type}.
+
+  Context `{Object Π Ω'}.
+
+  Variable Ω : Type.
+
+  Context `{Object Π Ω}.
 
   Fixpoint lift_term_r (e : Term.t Π Ω') : Term.t Π (Ω + Ω') :=
     match e with
@@ -325,10 +324,10 @@ Section Augmentation.
       ⟨ π , ψ , ϵ₂ , e ⟩ ⇓ₑ ⟨ ϵ₂' , v ⟩ →
         ⟨ π , ψ , disjoint_union ϵ₁ ϵ₂ , lift_term_r e ⟩ ⇓ₑ ⟨ disjoint_union ϵ₁ ϵ₂' , v ⟩.
   Proof.
-    induction e; intros; simpl in *; inv H3; try (econstructor; eauto).
+    induction e; intros; simpl in *; inv H1; try (econstructor; eauto).
     rewrite rebind_union_distr_r. econstructor.
       + eapply IHe. eauto.
-      + inv H10. econstructor. unfold Map.lookup in *. simpl in *. assumption.
+      + inv H8. econstructor. unfold Map.lookup in *. simpl in *. assumption.
   Qed.
 
   Lemma lift_term_r_sound_r :
@@ -336,12 +335,12 @@ Section Augmentation.
       ⟨ π , ψ , ϵ , lift_term_r e ⟩ ⇓ₑ ⟨ ϵ' , v ⟩ →
         ⟨ π , ψ , πᵣ ϵ , e ⟩ ⇓ₑ ⟨ πᵣ ϵ' , v ⟩.
   Proof.
-    induction e; intros; simpl in *; inv H3; try (econstructor; eauto).
+    induction e; intros; simpl in *; inv H1; try (econstructor; eauto).
     rewrite πᵣ_rebind_comm. econstructor.
     + apply IHe. eassumption.
-    + inv H10. constructor. simpl in *.
-      replace (Map.lookup ω0 (πᵣ ϵ0)) 
-          with (Map.lookup (inr ω0) ϵ0) by reflexivity.
+    + inv H8. constructor. simpl in *.
+      replace (Map.lookup ω (πᵣ ϵ0)) 
+          with (Map.lookup (inr ω) ϵ0) by reflexivity.
       assumption.
   Qed.
 
@@ -349,15 +348,18 @@ Section Augmentation.
     ∀ e π ψ ϵ v ϵ',
       ⟨ π , ψ , ϵ , lift_term_r e ⟩ ⇓ₑ ⟨ ϵ' , v ⟩ → πₗ ϵ = πₗ ϵ'.
   Proof.
-    induction e; intros; simpl in *; inv H3; intuition.
-    - apply IHe in H9. subst. simpl in *.
-      replace (πₗ ϵ0) with (πₗ ϵ'0).
-      + apply rebind_r_πₗ.
-    - apply IHe1 in H7. apply IHe2 in H10. congruence.
-    - inv H9. eauto.
-    - apply IHe1 in H6. apply IHe2 in H9. congruence.
-    - apply IHe in H5. assumption.
-    - apply IHe in H5. assumption.
+    induction e; intros; simpl in *; inv H1; intuition.
+    - apply IHe in H7. simpl in *.
+      replace (πₗ ϵ0) with (πₗ ϵ'0).  apply rebind_r_πₗ.
+    - etransitivity.
+      + eapply IHe1. eassumption.
+      + eapply IHe2. eassumption.
+    - inv H7. eauto.
+    - etransitivity.
+      + eapply IHe1. eassumption.
+      + eapply IHe2. eassumption.
+    - eapply IHe. eassumption.
+    - eapply IHe. eassumption.
   Qed.
 
   Fixpoint lift_stmt_r (s : Stmt.t Π Ω') : Stmt.t Π (Ω + Ω') :=
@@ -377,7 +379,7 @@ Section Augmentation.
         ∀ ϵ₁,
           ⟨ π , ψ , disjoint_union ϵ₁ ϵ₂ , lift_stmt_r s ⟩ ⇓ₛ ⟨ ψ' , disjoint_union ϵ₁ ϵ₂' , sig ⟩.
   Proof.
-    intros. generalize dependent ϵ₁. induction H3; intros.
+    intros. generalize dependent ϵ₁. induction H1; intros.
     - econstructor.
     - econstructor. fold lift_stmt_r. eauto.
     - econstructor. eauto.
@@ -388,7 +390,7 @@ Section Augmentation.
       + fold lift_stmt_r. eapply IHeval.
     - econstructor. eapply lift_term_r_complete. eassumption.
     - econstructor.
-    - econstructor. eapply lift_term_r_complete in H3. eauto.
+    - econstructor. eapply lift_term_r_complete in H1. eauto.
     - econstructor. eapply lift_term_r_complete. eassumption.
   Qed.
 
@@ -398,19 +400,19 @@ Section Augmentation.
         ⟨ π , ψ , πᵣ ϵ , s ⟩ ⇓ₛ ⟨ ψ' , πᵣ ϵ' , sig ⟩.
   Proof.
     induction s; intros.
-    - inv H3; econstructor; eauto.
-    - inv H3. econstructor. eapply lift_term_r_sound_r. eassumption.
-    - inv H3.
+    - inv H1; econstructor; eauto.
+    - inv H1. econstructor. eapply lift_term_r_sound_r. eassumption.
+    - inv H1.
       + econstructor.
         * eapply lift_term_r_sound_r. eassumption.
         * eauto.
       + eapply eval_if_false.
         * eapply lift_term_r_sound_r. eassumption.
         * eauto.
-    - inv H3. econstructor.
-    - inv H3. econstructor. eapply lift_term_r_sound_r. assumption.
-    - simpl in *. destruct inv. inv H3. econstructor. eapply lift_term_r_sound_r. simpl. eassumption.
-    - inv H3. econstructor.
+    - inv H1. econstructor.
+    - inv H1. econstructor. eapply lift_term_r_sound_r. assumption.
+    - simpl in *. destruct inv. inv H1. econstructor. eapply lift_term_r_sound_r. simpl. eassumption.
+    - inv H1. econstructor.
   Qed.
 
   Lemma lift_stmt_r_sound_l :
@@ -418,29 +420,117 @@ Section Augmentation.
       ⟨ π , ψ , ϵ , lift_stmt_r s ⟩ ⇓ₛ ⟨ ψ' , ϵ' , sig ⟩ → πₗ ϵ = πₗ ϵ'.
   Proof.
     induction s; intros.
-    - inv H3.
+    - inv H1.
       + eauto.
       + eauto.
       + etransitivity.
         * eapply IHs1. eauto.
         * eauto.
-    - inv H3. reflexivity.
-    - inv H3.
+    - inv H1. reflexivity.
+    - inv H1.
       + etransitivity.
         * eapply lift_term_r_sound_l. eassumption.
         * eauto.
       + etransitivity.
         * eapply lift_term_r_sound_l. eassumption.
         * eauto.
-    - inv H3. econstructor.
-    - inv H3. eapply lift_term_r_sound_l. eassumption.
-    - cbn in *. destruct inv. inv H3. eapply lift_term_r_sound_l.
-      assert (@Term.Invoke _ (Ω + Ω') _ _ (inr ω0) op (lift_term_r arg) = lift_term_r (Term.Invoke ω0 op arg)) by reflexivity.
-      erewrite <- H3.
+    - inv H1. econstructor.
+    - inv H1. eapply lift_term_r_sound_l. eassumption.
+    - cbn in *. destruct inv. inv H1. eapply lift_term_r_sound_l.
+      assert (@Term.Invoke _ (Ω + Ω') _ _ (inr _) op (lift_term_r arg) = lift_term_r (Term.Invoke ω op arg)) by reflexivity.
+      erewrite <- H1.
       eassumption.
-    - inv H3. econstructor.
+    - inv H1. econstructor.
   Qed.
 
-  Definition augment := zip_with (λ l l', Seq (lift_stmt_l l) (lift_stmt_r l')).
-  
+End LiftR.
+
+(* Definition augment {Π Ω₀ Ω Ω' : Type} `{Object Π Ω₀, Object Π Ω, Object Π Ω'} {ω : Ω₀} (impl : Implementation Π Ω ω) (lines : (type ω).(OP) → list (Stmt.t Π Ω')) : Implementation Π (Ω + Ω') ω :=
+  {|
+    param := impl.(param)
+  |}.
+
+
+Definition augment {Π Ω Ω' : Type} `{Object Π Ω, Object Π Ω'} : list (Stmt.t Π Ω) → list (Stmt.t Π Ω') → list (Stmt.t Π (Ω + Ω')) :=
+  zip_with (λ l l', Seq (lift_stmt_l Ω' l) (lift_stmt_r Ω l')). *)
+
+Section Augmentation.
+
+  (* An augmentation specifies, f*)
+
+  Context {Π Ω₀ Ω} `{EqDecision Π, Object Π Ω₀, Object Π Ω} {ω : Ω}.
+
+  Variable impl : Implementation Π Ω ω.
+
+  Variant status :=
+    | Idle
+    | Pending (op : (type ω).(OP)) (arg : Value.t)
+    | Linearized (op : (type ω).(OP)) (arg : Value.t) (res : Value.t).
+
+  Variant pending : status → Prop := pending_intro op arg : pending (Pending op arg).
+
+  Definition atomic_configuration := ((type ω).(Σ) * (Π → status))%type.
+
+  (* A meta configuration relates states of the implemented object and the status of each process *)
+  Definition meta_configuration := (type ω).(Σ) → (Π → status) → Prop.
+
+  Variant meta_configurations := M.
+
+  Instance meta_config_eq_dec : EqDecision meta_configurations.
+  Proof. solve_decision. Defined.
+
+  Definition invoke (f : Π → status) π op arg := Map.rebind π (Pending op arg) f.
+
+  Inductive δ_many : (type ω).(Σ) → (Π → status) → list Π → (type ω).(Σ) → (Π → status) → Prop :=
+    | δ_many_refl σ f : δ_many σ f [] σ f
+    | δ_many_trans f σ π op arg σ' res πs σ'' f' :
+      (* if [π] has invoked [op(arg)], but not returned *)
+      f π = Pending op arg →
+      (* And (σ', res) ∈ δ(σ, π, op, arg) *)
+      (type ω).(δ) σ π op arg σ' res →
+      δ_many σ' (Map.rebind π (Linearized op arg res) f) πs σ'' f' →
+      δ_many σ f (π :: πs) σ'' f'.
+
+  Variant evolve_inv (C : meta_configuration) (op : (type ω).(OP)) (π : Π) (arg : Value.t) : meta_configuration :=
+    evolve_inv_intro σ f πs σ' f' :
+      (* If (σ, f) ∈ C *)
+      C σ f →
+      (* If every process in permutation [πs] is pending *)
+      Forall (λ π, pending (f π)) πs → 
+      (* And atomic configuration (σ', f') results after linearizing every outstanding operation of [πs] *)
+      δ_many σ (invoke f π op arg) πs σ' f' →
+      (* Then (σ', f') is in the resulting metaconfiguration *)
+      evolve_inv C op π arg σ' f'.
+
+  Variant transition_meta_config : meta_configuration → Π → (type ω).(OP) → Value.t → meta_configuration → Value.t → Prop :=
+    | transition_evolve_inv C π op arg : transition_meta_config C π op arg (evolve_inv C op π arg) Value.Unit.
+
+  Variant meta_config_operations := EvolveInv | Evolve | EvolveRet.
+
+  Instance object_meta_config : Object Π meta_configurations :=
+    λ M, 
+      {|
+        Σ := (type ω).(Σ) → (Π → status) → Prop;
+        OP := meta_config_operations * (type ω).(OP);
+        δ σ π op v σ' res := False;
+      |}.
+
 End Augmentation.
+
+  (* Auxillary objects *)
+  (* Variable Ω' : Type.
+
+  Context `{Object Π Ω'} := zip_with (λ l l', Seq (lift_stmt_l l) (lift_stmt_r l')).
+
+  (* Type of implemented object *)
+  Variable Ω₀ : Type.
+
+  (* The object being implemented *)
+  Variable ω : Ω₀.
+
+  Context `{Object Π Ω₀}.
+
+  Variable impl : Implementation Π Ω ω.
+
+  
+End Augmentation. *)
