theories/Object.v
@@ -9,16 +9,15 @@ Record object_type (Π : Type) := {
   δ : Σ → Π → OP → Value.t → Σ → Value.t → Prop;
 }.
 
-Class Object (Π : Type) (Ω : Type) `{EqDecision Ω} := {
-  type : Ω → object_type Π;
-  (* state : ∀ (ω : Ω), (type ω).(Σ Π) *)
-}.
+Arguments Σ {_}.
+Arguments OP {_}.
+Arguments δ {_}.
 
-Instance augmentation_Object (Ω Ω' Π : Type) `{Object Π Ω, Object Π Ω'} : Object Π (Ω + Ω') := {
-  type obj :=
+Class Object (Π : Type) (Ω : Type) `{EqDecision Ω} := type : Ω → object_type Π.
+
+Instance augmentation_Object (Ω Ω' Π : Type) `{Object Π Ω, Object Π Ω'} : Object Π (Ω + Ω') :=
+  λ obj,
     match obj with
     | inl ω => type ω
     | inr ω => type ω
-    end
-}.
-
+    end.
