theories/Syntax/Value.v
@@ -1,6 +1,5 @@
 From stdpp Require Import base gmap.
 Require Import Coq.Classes.SetoidDec.
-Require Import Coq.ZArith.BinInt.
 Require Import Coq.Lists.List.
 Require Import Coq.Logic.Decidable.
 
